\documentclass{article}
\usepackage{amsfonts} 
\usepackage{pst-3dplot} 
\title{Assignment 1: Problem 1}
\author{Ernesto Rodriguez}
\begin{document}
\maketitle

\section{Notation}

Zero or first unary natural number: 0
Successor of n: s(n)
Multiple successor operatios: sss(n), equals to the successor of the succesor of the successor of n.

\section{Solution}

\begin{enumerate}

  {\item {\bf Base Case:}

    $a + b = b + a, b=0$ 

    $a+0=0+a$ 

    $a=0+a$ 

    $a+0=0+a+0$

    $a=0+a$ 

    {\bf Step Case: }

    $a+b=b+a$

    $s(a+b)=s(b+a)$

    $a+s(b)=b+s(a)$

    $a+b+s(0)=b+a+s(0)$ , a+b=b+a So we have: 

    $s(0)=s(0)$
    }

  {\item {\bf Base Case:} 

    $(a+b) * c = a*c + b*c$ ,c=0

    $(a+b) * 0 = a*0 + b*0$

    $(a+b) * 0 = 0$

    {\bf Step Case:}

    $(a+b) * c = a*c + b*c$ ,c=s(c)

    $(a+b) * s(c) = a*s(c) + b*s(c)$

    $(a+b) + (a+b)*s(c) = a + a*c + b + b*c$

    $a+b+a*c+b+b*c=a+a*c+b+b*c$
    }

  {\item {\bf Base Case:}

    $a*0=0*a$

    $a*s(0)=s(0)*a$

    $a+a*0=s(0)*a$

    $a=s(0)*a$

    {\bf Step Case:}

    $a*s(b)=s(b)*a$

    $a*(b+s(0))=(b+s(0))*a$

    $a*b + a*s(0)=b*a +s(0)*a$

    $a*b=b*a$ and $a*s(0)=s(0)*a$
    
  }

  \end{enumerate}

\end{document}
