\documentclass{article}
\usepackage{amsfonts}
\usepackage{graphicx}
\usepackage{mathtools}
\title{Assignment 5: ADT's, Inductive Functions and SML}
\author{Ernesto Rodriguez}
\begin{document}
\maketitle

\section{Problem 1}

The statement says that if x,y are coprime we can find an a,b such that $a<y$ and $b<x$ and:

\begin{equation}
  a*x-b*y=1
\end{equation}

Now assume $a>y$ and $b>x$ now we have:

\[
a*x-b*y=1 
\]
\[
a*x-1=b*y
\]
\begin{equation}
\frac{a*x}{b}-\frac{1}{b}=y
\end{equation}

Since we assume $b>x$ from equation 2 we can deduce that:

\[
\frac{a}{b}-\frac{1}{b}\leq\frac{a*x}{b}-\frac{1}{b}=y
\]
\[
\frac{a}{b}-\frac{1}{b}\leq y
\]
\[
\frac{a}{b}\leq y+\frac{1}{b}
\]

Since $b\geq1$ we have:
\[
y \leq y+\frac{1}{b}
\]

This implies that:

\[
\frac{a}{b}\leq y
\]
\begin{equation}
  a\leq b*y
\end{equation}

We know $b\geq1$ so we also know that:

\[
y\leq y*b
\]

Thus we can rewrite equation 3 as:
\begin{equation}
  a \leq y
\end{equation}

Which is a contradiction to the original assumption that $y>a$.

\end{document}
